STLC/Ela.v
@@ -52,81 +52,111 @@ Proof.
     reflexivity.
 Qed.
 
-Fixpoint elab_infer (g : ctx) (s : string -> option (hidden (db g))) (e : ast) {struct e} : option (hidden (tm g))
-  with elab_check (g : ctx) (s : string -> option (hidden (db g))) (e : ast) (t : tp) {struct e} : option (tm g t).
+Inductive elabres (T : Type) : Type :=
+  | Ok : T -> elabres T
+  | UndefName : string -> elabres T
+  | NeedAnnot : elabres T
+  | WrongType : elabres T.
+
+Fixpoint elab_infer (g : ctx) (s : string -> option (hidden (db g))) (e : ast) {struct e} : elabres (hidden (tm g))
+  with elab_check (g : ctx) (s : string -> option (hidden (db g))) (e : ast) (t : tp) {struct e} : elabres (tm g t).
 Proof.
   - (* defining elab_infer *)
     destruct e.
     * (* EVar *)
       destruct (s s0) as [[t n]|].
-      apply (Some (Ev _ t (Var _ _ n))).
-      apply None.
+      apply (Ok _ (Ev _ t (Var _ _ n))).
+      apply (UndefName _ s0).
     * (* ELam *)
       destruct o as [ta|].
-      + destruct (elab_infer _ (weaken_s _ s s0 ta) e) as [[tr body]|].
-        apply (Some (Ev _ (TArr ta tr) (Lam _ _ _ body))).
-        apply None.
-      + apply None. (* lack of info, give up *)
+      destruct (elab_infer _ (weaken_s _ s s0 ta) e) as [[tr body]|err| | ].
+      apply (Ok _ (Ev _ (TArr ta tr) (Lam _ _ _ body))).
+      apply (UndefName _ err).
+      apply NeedAnnot.
+      apply WrongType.
+      apply NeedAnnot.
     * (* EApp *)
-      destruct (elab_infer _ s e1) as [[[ta tr| |c1 c2|i1 i2] tm1]|].
+      destruct (elab_infer _ s e1) as [[[ta tr| |c1 c2|i1 i2] tm1]|err| |].
       + (* we inferred e1 as ta -> tr *)
-        destruct (elab_check _ s e2 ta) as [tm2|].
-        apply (Some (Ev _ tr (App _ _ _ tm1 tm2))).
-        apply None.
-      + apply None. (* a whole bunch of type-mismatch cases *)
-      + apply None.
-      + apply None.
-      + (* we couldn't infer e1 *)
-        apply None.
+        destruct (elab_check _ s e2 ta) as [tm2|err| |].
+        apply (Ok _ (Ev _ tr (App _ _ _ tm1 tm2))).
+        apply (UndefName _ err).
+        apply NeedAnnot.
+        apply WrongType.
+      + apply WrongType.
+      + apply WrongType.
+      + apply WrongType.
+      + apply (UndefName _ err).
+      + apply NeedAnnot.
+      + apply WrongType.
     * (* EUnit *)
-      apply (Some (Ev _ TUnit (Unit _))).
+      apply (Ok _ (Ev _ TUnit (Unit _))).
     * (* ELet *)
-      destruct (elab_infer _ s e1) as [[t1 tm1]|].
+      destruct (elab_infer _ s e1) as [[t1 tm1]|err| | ].
       + (* we inferred e1 *)
-        destruct (elab_infer _ (weaken_s _ s s0 t1) e2) as [[t2 tm2]|].
-        apply (Some (Ev _ t2 (Let _ _ _ tm1 tm2))).
-        apply None.
-      + (* we couldn't infer e1 *)
-        apply None.
+        destruct (elab_infer _ (weaken_s _ s s0 t1) e2) as [[t2 tm2]|err| |].
+        apply (Ok _ (Ev _ t2 (Let _ _ _ tm1 tm2))).
+        apply (UndefName _ err).
+        apply NeedAnnot.
+        apply WrongType.
+      + apply (UndefName _ err).
+      + apply NeedAnnot.
+      + apply WrongType.
     * (* EPair *)
-      destruct (elab_infer _ s e1) as [[t1 tm1]|].
-      destruct (elab_infer _ s e2) as [[t2 tm2]|].
-      apply (Some (Ev _ (TPair t1 t2) (Pair _ _ _ tm1 tm2))).
-      apply None.
-      apply None.
+      destruct (elab_infer _ s e1) as [[t1 tm1]|err| |].
+      destruct (elab_infer _ s e2) as [[t2 tm2]|err| |].
+      apply (Ok _ (Ev _ (TPair t1 t2) (Pair _ _ _ tm1 tm2))).
+      apply (UndefName _ err).
+      apply NeedAnnot.
+      apply WrongType.
+      apply (UndefName _ err).
+      apply NeedAnnot.
+      apply WrongType.
     * (* EFst *)
-      destruct (elab_infer _ s e) as [[[_1 _2| |t1 t2|i1 i2] tm]|].
-      apply None.
-      apply None.
-      apply (Some (Ev _ t1 (Fst _ _ _ tm))).
-      apply None.
-      apply None.
+      destruct (elab_infer _ s e) as [[[_1 _2| |t1 t2|i1 i2] tm]|err| |].
+      apply WrongType.
+      apply WrongType.
+      apply (Ok _ (Ev _ t1 (Fst _ _ _ tm))).
+      apply WrongType.
+      apply (UndefName _ err).
+      apply NeedAnnot.
+      apply WrongType.
     * (* ESnd *)
-      destruct (elab_infer _ s e) as [[[_1 _2| |t1 t2|i1 i2] tm]|].
-      apply None.
-      apply None.
-      apply (Some (Ev _ t2 (Snd _ _ _ tm))).
-      apply None.
-      apply None.
+      destruct (elab_infer _ s e) as [[[_1 _2| |t1 t2|i1 i2] tm]|err| |].
+      apply WrongType.
+      apply WrongType.
+      apply (Ok _ (Ev _ t2 (Snd _ _ _ tm))).
+      apply WrongType.
+      apply (UndefName _ err).
+      apply NeedAnnot.
+      apply WrongType.
     * (* EInl *)
-      apply None. (* don't know what type to assign to the other entry. *)
+      apply NeedAnnot.
     * (* EInr *)
-      apply None.
+      apply NeedAnnot.
     * (* ECase *)
-      destruct (elab_infer _ s e1) as [[[_1 _2| |c1 c2|i1 i2] tm1]|].
-      apply None.
-      apply None.
-      apply None.
-      destruct (elab_infer _ (weaken_s _ s s0 i1) e2) as [[tr tm2]|].
-      destruct (elab_check _ (weaken_s _ s s0 i2) e3 tr) as [tm3|].
-      apply (Some (Ev _ tr (Case _ _ _ _ tm1 tm2 tm3))).
-      apply None.
-      apply None.
-      apply None.
+      destruct (elab_infer _ s e1) as [[[_1 _2| |c1 c2|i1 i2] tm1]|err| |].
+      apply WrongType.
+      apply WrongType.
+      apply WrongType.
+      destruct (elab_infer _ (weaken_s _ s s0 i1) e2) as [[tr tm2]|err| |].
+      destruct (elab_check _ (weaken_s _ s s0 i2) e3 tr) as [tm3|err| |].
+      apply (Ok _ (Ev _ tr (Case _ _ _ _ tm1 tm2 tm3))).
+      apply (UndefName _ err).
+      apply NeedAnnot.
+      apply WrongType.
+      apply (UndefName _ err).
+      apply NeedAnnot.
+      apply WrongType.
+      apply (UndefName _ err).
+      apply NeedAnnot.
+      apply WrongType.
     * (* EAnn *)
       destruct (elab_check _ s e t).
-      apply (Some (Ev _ t t0)).
-      apply None.
+      apply (Ok _ (Ev _ t t0)).
+      apply (UndefName _ s0).
+      apply NeedAnnot.
+      apply WrongType.
 
   - (* defining elab_check *)
     destruct e.
@@ -134,108 +164,137 @@ Proof.
       destruct (s s0) as [[t0 n]|].
       + (* variable exists *)
         destruct (tp_eq_dec t0 t).
-        rewrite <- e. apply (Some (Var _ _ n)).
-        apply None.
+        rewrite <- e. apply (Ok _ (Var _ _ n)).
+        apply WrongType.
       + (* variable does not exist *)
-        apply None.
+        apply (UndefName _ s0).
     * (* ELam *)
       destruct t as [ta tr| | c1 c2|i1 i2].
       + (* ta -> tr *)
         destruct o as [ta'|].
         ++ destruct (tp_eq_dec ta' ta).
-           +++ destruct (elab_check _ (weaken_s _ s s0 ta) e tr) as [body|].
-               apply (Some (Lam _ _ _  body)).
-               apply None.
-           +++ apply None.
-        ++ destruct (elab_check _ (weaken_s _ s s0 ta) e tr) as [body|].
-           apply (Some (Lam _ _ _  body)).
-           apply None.
-      + apply None. (* a whole bunch of type-mismatch cases *)
-      + apply None.
-      + apply None.
+           destruct (elab_check _ (weaken_s _ s s0 ta) e tr) as [body|err| |].
+           apply (Ok _ (Lam _ _ _  body)).
+           apply (UndefName _ err).
+           apply NeedAnnot.
+           apply WrongType.
+           apply WrongType.
+        ++ destruct (elab_check _ (weaken_s _ s s0 ta) e tr) as [body|err| |].
+           apply (Ok _ (Lam _ _ _  body)).
+           apply (UndefName _ err).
+           apply NeedAnnot.
+           apply WrongType.
+      + apply WrongType. (* a whole bunch of type-mismatch cases *)
+      + apply WrongType.
+      + apply WrongType.
     * (* EApp *)
-      destruct (elab_infer _ s e1) as [[[ta tr| | c1 c2|i1 i2] tm1]|].
+      destruct (elab_infer _ s e1) as [[[ta tr| | c1 c2|i1 i2] tm1]|err| |].
       + (* we inferreed e1 as ta -> tr *)
         destruct (tp_eq_dec tr t).
-        ++ destruct (elab_check _ s e2 ta) as [tm2|].
-           rewrite <- e. apply (Some (App _ _ _ tm1 tm2)).
-           apply None.
-        ++ apply None.
-      + apply None. (* a whole bunch of type-mismatch cases *)
-      + apply None.
-      + apply None.
-      + apply None.
+        ++ destruct (elab_check _ s e2 ta) as [tm2|err| |].
+           rewrite <- e. apply (Ok _ (App _ _ _ tm1 tm2)).
+           apply (UndefName _ err).
+           apply NeedAnnot.
+           apply WrongType.
+        ++ apply WrongType.
+      + apply WrongType. (* a whole bunch of type-mismatch cases *)
+      + apply WrongType.
+      + apply WrongType.
+      + apply (UndefName _ err).
+      + apply NeedAnnot.
+      + apply WrongType.
     * (* EUnit *)
       destruct (tp_eq_dec TUnit t).
-      rewrite <- e. apply (Some (Unit _)).
-      apply None.
+      rewrite <- e. apply (Ok _ (Unit _)).
+      apply WrongType.
     * (* ELet *)
-      destruct (elab_infer _ s e1) as [[t1 tm1]|].
+      destruct (elab_infer _ s e1) as [[t1 tm1]|err| |].
       + (* we inferred e1 *)
-        destruct (elab_check _ (weaken_s _ s s0 t1) e2 t) as [tm2|].
-        apply (Some (Let _ _ _ tm1 tm2)).
-        apply None.
-      + (* we couldn't infer e'1 *)
-        apply None.
+        destruct (elab_check _ (weaken_s _ s s0 t1) e2 t) as [tm2|err| |].
+        apply (Ok _ (Let _ _ _ tm1 tm2)).
+        apply (UndefName _ err).
+        apply NeedAnnot.
+        apply WrongType.
+      + apply (UndefName _ err).
+      + apply NeedAnnot.
+      + apply WrongType.
     * (* EPair *)
       destruct t as [_1 _2| |t1 t2|i1 i2].
-      + apply None.
-      + apply None.
+      + apply WrongType.
+      + apply WrongType.
       + (* t1 * t2 *)
-        destruct (elab_check _ s e1 t1) as [tm1|].
-        destruct (elab_check _ s e2 t2) as [tm2|].
-        apply (Some (Pair _ _ _ tm1 tm2)).
-        apply None.
-        apply None.
-      + apply None.
+        destruct (elab_check _ s e1 t1) as [tm1|err| |].
+        destruct (elab_check _ s e2 t2) as [tm2|err| |].
+        apply (Ok _ (Pair _ _ _ tm1 tm2)).
+        apply (UndefName _ err).
+        apply NeedAnnot.
+        apply WrongType.
+        apply (UndefName _ err).
+        apply NeedAnnot.
+        apply WrongType.
+      + apply WrongType.
     * (* EFst *)
-      destruct (elab_infer _ s e) as [[[_1 _2| |t1 t2|i1 i2] tm]|].
-      apply None.
-      apply None.
+      destruct (elab_infer _ s e) as [[[_1 _2| |t1 t2|i1 i2] tm]|err| |].
+      apply WrongType.
+      apply WrongType.
       destruct (tp_eq_dec t1 t).
-      rewrite <- e0. apply (Some (Fst _ _ _ tm)).
-      apply None.
-      apply None.
-      apply None.
+      rewrite <- e0. apply (Ok _ (Fst _ _ _ tm)).
+      apply WrongType.
+      apply WrongType.
+      apply (UndefName _ err).
+      apply NeedAnnot.
+      apply WrongType.
     * (* ESnd *)
-      destruct (elab_infer _ s e) as [[[_1 _2| |t1 t2|i1 i2] tm]|].
-      apply None.
-      apply None.
+      destruct (elab_infer _ s e) as [[[_1 _2| |t1 t2|i1 i2] tm]|err| |].
+      apply WrongType.
+      apply WrongType.
       destruct (tp_eq_dec t2 t).
-      rewrite <- e0. apply (Some (Snd _ _ _ tm)).
-      apply None.
-      apply None.
-      apply None.
+      rewrite <- e0. apply (Ok _ (Snd _ _ _ tm)).
+      apply WrongType.
+      apply WrongType.
+      apply (UndefName _ err).
+      apply NeedAnnot.
+      apply WrongType.
     * (* EInl *)
       destruct t as [ta tr| |c1 c2|i1 i2].
-      apply None.
-      apply None.
-      apply None.
-      destruct (elab_check _ s e i1) as [tm|].
-      + apply (Some (Inl _ _ _ tm)).
-      + apply None.
+      apply WrongType.
+      apply WrongType.
+      apply WrongType.
+      destruct (elab_check _ s e i1) as [tm|err| |].
+      + apply (Ok _ (Inl _ _ _ tm)).
+      + apply (UndefName _ err).
+      + apply NeedAnnot.
+      + apply WrongType.
     * (* EInr *)
       destruct t as [ta tr| |c1 c2|i1 i2].
-      apply None.
-      apply None.
-      apply None.
-      destruct (elab_check _ s e i2) as [tm|].
-      + apply (Some (Inr _ _ _ tm)).
-      + apply None.
+      apply WrongType.
+      apply WrongType.
+      apply WrongType.
+      destruct (elab_check _ s e i2) as [tm|err| |].
+      + apply (Ok _ (Inr _ _ _ tm)).
+      + apply (UndefName _ err).
+      + apply NeedAnnot.
+      + apply WrongType.
     * (* ECase *)
-      destruct (elab_infer _ s e1) as [[[_1 _2| |c1 c2|i1 i2] tm1]|].
-      apply None.
-      apply None.
-      apply None.
-      destruct (elab_check _ (weaken_s _ s s0 i1) e2 t) as [tm2|].
-      destruct (elab_check _ (weaken_s _ s s0 i2) e3 t) as [tm3|].
-      apply (Some (Case _ _ _ _ tm1 tm2 tm3)).
-      apply None.
-      apply None.
-      apply None.
+      destruct (elab_infer _ s e1) as [[[_1 _2| |c1 c2|i1 i2] tm1]|err| |].
+      apply WrongType.
+      apply WrongType.
+      apply WrongType.
+      destruct (elab_check _ (weaken_s _ s s0 i1) e2 t) as [tm2|err| |].
+      destruct (elab_check _ (weaken_s _ s s0 i2) e3 t) as [tm3|err| |].
+      apply (Ok _ (Case _ _ _ _ tm1 tm2 tm3)).
+      apply (UndefName _ err).
+      apply NeedAnnot.
+      apply WrongType.
+      apply (UndefName _ err).
+      apply NeedAnnot.
+      apply WrongType.
+      apply (UndefName _ err).
+      apply NeedAnnot.
+      apply WrongType.
     * (* EAnn *)
       destruct (tp_eq_dec t0 t).
       rewrite <- e0. apply (elab_check _ s e t0).
-      apply None.
+      apply WrongType.
 Defined.
 
